A12Kernel.lean
@@ -117,6 +117,7 @@ import A12Kernel.Elaboration.IndexedDateRangeConstructionComputation
 import A12Kernel.Elaboration.DateRangeBound
 import A12Kernel.Elaboration.DateRangeStoredComparison
 import A12Kernel.Elaboration.YearlessDateRangeBound
+import A12Kernel.Elaboration.DateRangeBoundComparison
 import A12Kernel.Elaboration.DateRangeOverlap
 import A12Kernel.Elaboration.AtLeastOneDateRangeOverlap
 import A12Kernel.Elaboration.YearlessDateRangeOverlap
